theories/opsem_systemF_ctx.v
@@ -254,6 +254,252 @@ Proof.
   inversion step2; subst.
 Admitted.
 
+Lemma step_fill K : forall e e',
+    e ~> e' ->
+    fill K e ~> fill K e'.
+Proof.
+  intros.
+  inversion H; subst.
+  rewrite! fill_comp.
+  eapply Step; eauto.
+Qed.
+
+Lemma mstep_fill K : forall e e',
+  e ~>* e' ->
+  fill K e ~>* fill K e'.
+Proof.
+  intros. generalize dependent K.
+  induction H; intros.
+  + apply star_refl.
+  + apply (step_fill K) in H.
+    eapply star_step; eauto.
+    apply IHstar.
+Qed.
+
+Definition is_val_dec :
+  ∀ e, is_val e ∨ ¬ is_val e.
+Proof.
+   induction e; try (by right; inversion 1).
+   - left; constructor.
+   - destruct IHe1; [|by right; inversion 1].
+     destruct IHe2; [|by right; inversion 1].
+     by left; constructor.
+   - left; constructor.
+   - left; constructor.
+Qed.
+
+Lemma is_val_fill K e :
+  is_val (fill K e) -> is_val e.
+Proof.
+  intros.
+  induction K; inversion H; cbn in *; subst;auto.
+Qed.
+
+(* If pure step from (fill K e), then either
+   - e is a value
+   - K is empty
+ *)
+Lemma pure_step_fill :
+∀ K e e', (fill K e) -h-> e' → (∀ e'', (fill K e'') = e'') ∨ is_val e.
+Proof.
+  induction K;intros.
+  - (* Empty *)
+    left; cbn in *;intros;auto.
+  - (* Fst *)
+    destruct K; inversion H; subst; right.
+    econstructor; eauto.
+    by eapply is_val_fill.
+    by eapply is_val_fill.
+  - (* Snd *)
+    destruct K; inversion H; subst; right.
+    econstructor; eauto.
+    by eapply is_val_fill.
+    by eapply is_val_fill.
+  - (* PairL *)
+    destruct K; inversion H; subst; right.
+  - (* PairR *)
+    destruct K; inversion H; subst; right.
+  - (* AppL *)
+    destruct K; inversion H; subst; right; constructor.
+  - (* AppR *)
+    inversion H; subst; right.
+    by eapply is_val_fill.
+  - (* TApp *)
+    destruct K; inversion H; subst; right; constructor.
+Qed.
+
+Lemma of_val_injective : forall e1 e2,
+of_val e1 = of_val e2 -> e1 = e2.
+Proof.
+  induction e1; intros; destruct e2;cbn in H; auto; try discriminate;injection H
+  ;intros.
+  - apply IHe1_1 in H1;subst.
+    apply IHe1_2 in H0;subst.
+    reflexivity.
+  - by subst.
+  - by subst.
+Qed.
+
+Lemma ectx_decompose K1 K2 e1 e2 :
+  (fill K1 e1) = (fill K2 e2) →
+  ¬ is_val e1 →
+  ¬ is_val e2 →
+  (∃ K3, forall e3, (fill K1 e3) = (fill K2 (fill K3 e3)))
+  ∨ (∃ K3, forall e3, (fill K2 e3) = (fill K1 (fill K3 e3))).
+Proof.
+  revert e1 e2 K2.
+  induction K1; intros e1 e2 K2 Heq Hnv1 Hnv2; cbn in Heq.
+  - (* EmptyCtx *)
+    right. by exists K2; intros e3; cbn.
+  - (* FstCtx *)
+     destruct K2.
+     all: try (by left; exists (FstCtx K1); cbn in *; auto).
+     cbn in *.
+     injection Heq; intro HeqK.
+     apply IHK1 in HeqK; auto.
+     destruct HeqK as [(K3 & HeqK)|(K3 & HeqK)]
+     ;[left|right]; exists K3; intros; by rewrite HeqK.
+  - (* SndCtx *)
+     destruct K2.
+     all: try (by left; exists (SndCtx K1); cbn in *; auto).
+     cbn in *.
+     injection Heq; intro HeqK.
+     apply IHK1 in HeqK; auto.
+     destruct HeqK as [(K3 & HeqK)|(K3 & HeqK)]
+     ;[left|right]; exists K3; intros; by rewrite HeqK.
+  - (* LPairCtx *)
+     destruct K2.
+     all: try (by left; exists (LPairCtx K1 e); cbn in *; auto).
+     + cbn in *.
+       injection Heq; intros -> HeqK.
+       apply IHK1 in HeqK; auto.
+       destruct HeqK as [(K3 & HeqK)|(K3 & HeqK)]
+       ;[left|right]; exists K3; intros; by rewrite HeqK.
+     + cbn in *.
+       injection Heq; intros -> HeqK.
+       pose proof (is_val_of_val v) as contra.
+       rewrite <- HeqK in contra.
+       apply is_val_fill in contra. contradiction.
+  - (* RPairCtx *)
+     destruct K2.
+     all: try (by left; exists (RPairCtx K1 v); cbn in *; auto).
+     + cbn in *.
+       injection Heq; intros <- HeqK.
+       pose proof (is_val_of_val v) as contra.
+       rewrite HeqK in contra.
+       apply is_val_fill in contra. contradiction.
+     + cbn in *.
+       injection Heq; intros HeqK HeqV.
+       apply of_val_injective in HeqV ; subst.
+       apply IHK1 in HeqK; auto.
+       destruct HeqK as [(K3 & HeqK)|(K3 & HeqK)]
+       ;[left|right]; exists K3; intros; by rewrite HeqK.
+  - (* LAppCtx *)
+     destruct K2.
+     all: try (by left; exists (LAppCtx K1 e); cbn in *; auto).
+     + cbn in *.
+       injection Heq; intros <- HeqK.
+       apply IHK1 in HeqK; auto.
+       destruct HeqK as [(K3 & HeqK)|(K3 & HeqK)]
+       ;[left|right]; exists K3; intros; by rewrite HeqK.
+     + cbn in *.
+       injection Heq; intros -> HeqK.
+       pose proof (is_val_of_val v) as contra.
+       rewrite <- HeqK in contra.
+       apply is_val_fill in contra; contradiction.
+  - (* RAppCtx *)
+     destruct K2.
+     all: try (by left; exists (RAppCtx K1 v); cbn in *; auto).
+     + cbn in *.
+       injection Heq; intros <- HeqK.
+       pose proof (is_val_of_val v) as contra.
+       rewrite HeqK in contra.
+       apply is_val_fill in contra; contradiction.
+     + cbn in *.
+       injection Heq; intros HeqK HeqV.
+       apply of_val_injective in HeqV ; subst.
+       apply IHK1 in HeqK; auto.
+       destruct HeqK as [(K3 & HeqK)|(K3 & HeqK)]
+       ;[left|right]; exists K3; intros; by rewrite HeqK.
+  - (* TAppCtx *)
+     destruct K2.
+     all: try (by left; exists (TAppCtx K1); cbn in *; auto).
+     cbn in *.
+     injection Heq; intros HeqK.
+     apply IHK1 in HeqK; auto.
+     destruct HeqK as [(K3 & HeqK)|(K3 & HeqK)]
+     ;[left|right]; exists K3; intros; by rewrite HeqK.
+Qed.
+
+Lemma fill_K_injective K : forall e e',
+ fill K e = fill K e' -> e = e'.
+Proof.
+  intros.
+  induction K;cbn in *;auto;apply IHK; by injection H.
+Qed.
+
+
+Lemma step_ectx (K : ectx) e e' :
+    (fill K e) ~> e' →
+    (is_val e) ∨ (∃ e'', e ~> e'' ∧ e' = (fill K e'')).
+Proof.
+  intros Hstep.
+  destruct (is_val_dec e) ; [left|right]; auto.
+  inversion Hstep as [K' e1 e2 HeqK ? Hpstep]; subst.
+  pose proof HeqK as HeqK0.
+  apply ectx_decompose in HeqK;[|assumption| ];cycle 1.
+  - intro contra. apply (is_val_stuck _ e2) in contra. apply contra.
+    by apply pure_contextual_step.
+  - destruct HeqK as [ ( K'' & HeqK ) | ( K'' & HeqK )]
+    ; rewrite HeqK in Hstep.
+    + rewrite HeqK in HeqK0.
+      apply fill_K_injective in HeqK0.
+      subst.
+      pose proof Hpstep as Hpstep2.
+      apply pure_step_fill in Hpstep.
+      destruct Hpstep.
+      * rewrite H0 in Hstep.
+        rewrite H0 in Hpstep2.
+        exists e2.
+        split; [by apply pure_contextual_step|].
+        rewrite HeqK.
+        by rewrite H0.
+      * tauto. (* TODO why does tauto work here ? *)
+    + rewrite HeqK in HeqK0.
+      apply fill_K_injective in HeqK0.
+      exists (fill K'' e2); split; [| by rewrite HeqK].
+      eapply Step;eauto.
+Qed.
+
+Lemma mstep_ectx (K : ectx) e e' :
+    (fill K e) ~>* e' →
+    (∃ e'', e' = (fill K e'') ∧ e ~>* e'')
+    ∨ (∃ v , is_val v ∧ e ~>* v ∧ (fill K v) ~>* e').
+Proof.
+  intros.
+  (* induction H. *)
+  (* - induction e. *)
+  (*   destruct (is_val_dec a). *)
+  (*   + (* a is a value *) *)
+  (*     right. exists a. *)
+  (*     pose proof pure_step_fill. *)
+  (* - destruct IHstar as [(e'' & -> & Hstep) | (v& Hval & Hmstep & Hstep)] *)
+  (*   ; [left; exists e'' |right ; exists v]; firstorder. *)
+  inversion H;subst.
+  - left. exists e. split;auto;constructor.
+  - apply step_ectx in H0.
+    destruct H0 as [Hv | (e'' & Hstep & ->)].
+    + right. exists e; firstorder. constructor.
+    + left. exists e; firstorder. 2: constructor.
+      (* TODO I finally end up in the same issue than previously
+         e --->* ef
+         |       ^*
+         v       |
+         e' -----|
+         which is true because determinism
+         but I don't know how to prove it, because the reflexive path does not give anything. *)
+Admitted.
+
 #[export]
   Hint Resolve
   cstep_app_l
